copy ca from direct refinement

process/Load.v
@@ -6,9 +6,142 @@ Require Import Lifting Encapsulation.
 
 Require Import List Maps.
 Import ListNotations.
-Require Import Machregs Asm.
+Require Import Conventions Mach Asm.
 
 Require Import InitMem With.
+
+(* Conventions.cc_c_locset @ cc_locset_mach @ cc_mach_asm *)
+
+Section CA.
+  Require Import Locations CallConv.
+
+  Record cc_ca_world :=
+    caw {
+        caw_sg : signature;
+        caw_rs : regset;
+        caw_m : mem
+      }.
+
+  Definition make_locset_rs (rs: regset) (m:mem) (sp: val) (l:loc):=
+    match l with
+    |R r => rs (preg_of r)
+    |S Outgoing ofs ty =>
+       let v := load_stack m sp ty (Ptrofs.repr (Stacklayout.fe_ofs_arg + 4 * ofs)) in Val.maketotal v
+    |_ => Vundef
+    end.
+
+  Inductive cc_c_asm_mq : cc_ca_world -> c_query -> query li_asm -> Prop:=
+    cc_c_asm_mq_intro sg args m (rs: regset) tm (ls : Locmap.t):
+      let sp := rs#SP in
+      let ra := rs#RA in
+      let vf := rs#PC in
+      args = (map (fun p => Locmap.getpair p ls) (loc_arguments sg)) ->
+      ls = make_locset_rs rs tm sp ->
+      args_removed sg sp tm m ->
+      Val.has_type sp Tptr ->
+      Val.has_type ra Tptr ->
+      valid_blockv (Mem.nextblock tm) sp ->
+      vf <> Vundef -> ra <> Vundef ->
+      cc_c_asm_mq
+        (caw sg rs tm)
+        (cq vf sg args m)
+        (rs,tm).
+
+  Definition rs_getpair (p: rpair preg) (rs : regset) :=
+    match p with
+    |One r => rs r
+    |Twolong r1 r2 => Val.longofwords (rs r1) (rs r2)
+    end.
+
+  Inductive cc_c_asm_mr : cc_ca_world -> c_reply -> reply li_asm -> Prop :=
+    cc_c_asm_mr_intro sg res tm m' tm' (rs rs' :regset) :
+      let sp := rs#SP in
+      res = rs_getpair (map_rpair preg_of (loc_result sg)) rs' ->
+      (forall r, is_callee_save r = true -> rs' (preg_of r) = rs (preg_of r)) ->
+      Mem.unchanged_on (not_init_args (size_arguments sg) sp) m' tm' ->
+      Mem.unchanged_on (loc_init_args (size_arguments sg) sp) tm tm' ->
+      Mem.nextblock m' = Mem.nextblock tm' ->
+      (forall b ofs k p, loc_init_args (size_arguments sg) sp b ofs ->
+                    ~ Mem.perm m' b ofs k p) ->
+      rs'#SP = rs#SP -> rs'#PC = rs#RA ->
+      cc_c_asm_mr
+        (caw sg rs tm)
+        (cr res m')
+        (rs', tm').
+
+  Program Definition cc_c_asm : callconv li_c li_asm :=
+    {|
+      match_senv _ := eq;
+      match_query := cc_c_asm_mq;
+      match_reply := cc_c_asm_mr
+    |}.
+  Next Obligation. reflexivity. Qed.
+  Next Obligation. inv H0. cbn. subst vf0. reflexivity. Qed.
+  Next Obligation. inv H. cbn. subst vf0. reflexivity. Qed.
+
+  Definition rs_to_mrs (rs : regset) := fun r: mreg => rs (preg_of r).
+
+  Require Import CallconvAlgebra.
+
+  Lemma cc_ca_cllmma :
+    ccref (cc_c_asm) (cc_c_locset @ cc_locset_mach @ cc_mach_asm).
+  Proof.
+    intros [sg rs tm] se1 se2 q1 q2 Hse. destruct Hse.
+    intros Hq. inversion Hq. subst sg0 rs0 tm0 q1 q2.
+    exists (se1,sg,(se1,(lmw sg (rs_to_mrs rs) tm sp),
+                (rs,Mem.nextblock tm))).
+    repeat apply conj; cbn in *; eauto.
+    - exists (lq vf sg ls m). split.
+      econstructor; eauto.
+      exists (mq vf sp ra (rs_to_mrs rs) tm). split. rewrite H3.
+      econstructor; eauto.
+      econstructor; eauto.
+    - intros cr ar [lr [Hr1 [mr [Hr2 Hr3]]]].
+      inv Hr1. inv Hr2. inv Hr3.
+      econstructor; eauto.
+      + destruct (loc_result sg).
+        -- simpl. rewrite <- H13. rewrite H9. reflexivity. simpl. auto.
+        -- simpl. f_equal.
+           rewrite <- H13. rewrite H9. reflexivity. simpl. eauto.
+           rewrite <- H13. rewrite H9. reflexivity. simpl. eauto.
+      + intros. rewrite <- H13. rewrite H12. reflexivity. eauto.
+  Qed.
+
+  Lemma cc_cllmma_ca :
+    ccref (cc_c_locset @ cc_locset_mach @ cc_mach_asm) (cc_c_asm).
+  Proof.
+    intros [[se' sg] [[se'' w2] [rs tm]]] se''' se q1 q2 Hse Hq.
+    destruct Hse. inv H. destruct H0. inv H. inv H0.
+    destruct Hq as [lq [Hq1 [mq [Hq2 Hq3]]]]. cbn in *.
+    inv Hq1. inv Hq2. inv Hq3.
+    rename rs1 into mrs. rename m0 into tm.
+    exists (caw sg rs tm).
+    repeat apply conj; eauto.
+    - econstructor; eauto.
+      apply Axioms.extensionality.
+      intro r. destruct r; simpl; eauto.
+    - intros r1 r2 Hr. inv Hr.
+      set (ls' loc :=
+             match loc with
+             |R r => rs' (preg_of r)
+             |_ => Vundef
+             end
+          ).
+      exists (lr ls'  m'). split.
+      constructor; eauto.
+      destruct (loc_result); simpl; eauto.
+      exists (mr (rs_to_mrs rs') tm'). split.
+      constructor; eauto.
+      intros. unfold rs_to_mrs. rewrite H3. eauto. eauto.
+      constructor; eauto.
+      inversion H8. eauto.
+  Qed.
+
+  Lemma ca_cllmma_equiv :
+    cceqv cc_c_asm (cc_c_locset @ cc_locset_mach @ cc_mach_asm).
+  Proof. split. apply cc_ca_cllmma. apply cc_cllmma_ca. Qed.
+
+End CA.
 
 Notation tint := (Tint I32 Unsigned noattr).
 
@@ -100,18 +233,60 @@ Section INIT_ASM.
     |}.
 End INIT_ASM.
 
+Section VA.
+
+  Require Import ValueDomain ValueAnalysis VAInject.
+
+  Context (se: Genv.symtbl) sk m (Hm: init_mem se sk = Some m).
+  Let bc := bc_of_symtbl se.
+
+  Lemma init_mem_block_classification:
+    genv_match bc se
+    /\ bc_below bc (Mem.nextblock m)
+    /\ bc_nostack bc
+    /\ (forall b id, bc b = BCglob id -> Genv.find_symbol se id = Some b)
+    /\ (forall b, Mem.valid_block m b -> bc b <> BCinvalid).
+  Admitted.
+
+  Lemma init_mem_matches:
+    forall cu, Genv.valid_for (erase_program cu) se -> romatch bc m (romem_for cu).
+  Proof.
+    intros. red. intros * Hb Hid.
+    assert (B: romem_consistent (prog_defmap cu) (romem_for cu))
+      by apply romem_for_consistent.
+  Admitted.
+
+End VA.
+
 Require Import Compiler.
 
 Section INIT_C_ASM.
 
   Local Transparent Archi.ptr64.
 
+  Lemma match_stbls_flat_inj se:
+    Genv.match_stbls (Mem.flat_inj (Genv.genv_next se)) se se.
+  Proof.
+    split; eauto; unfold Mem.flat_inj; intros.
+    - destruct plt; try easy. eexists. reflexivity.
+    - intros. unfold Mem.flat_inj. exists b2. destruct plt; try easy.
+    - destruct plt; try easy. inv H. reflexivity.
+    - destruct plt; try easy. inv H. reflexivity.
+    - destruct plt; try easy. inv H. reflexivity.
+  Qed.
+
+  Lemma match_prog_skel p tp:
+    match_prog p tp -> erase_program p = erase_program tp.
+  Proof.
+    intros. edestruct clight_semantic_preservation as [H1 ?]; eauto.
+    destruct H1. destruct X. apply fsim_skel.
+  Qed.
+
   Lemma init_c_asm p tp:
     match_prog p tp -> forward_simulation cc_compcert 1 (init_c p) (init_asm tp).
   Proof.
     intros H. assert (Hsk: erase_program p = erase_program tp).
-    { apply clight_semantic_preservation in H as [H1 ?].
-      apply H1. }
+    eapply match_prog_skel; eauto.
     constructor. econstructor. apply Hsk.
     intros. reflexivity.
     intros. instantiate (1 := fun _ _ _ => _). cbn beta. destruct H0.
@@ -169,19 +344,22 @@ Section INIT_C_ASM.
         (* cc_asm vainj *)
         instantiate (1 := (se1, Inject.injw (Mem.flat_inj (Mem.nextblock m)) (Mem.nextblock m) (Mem.nextblock m))).
         repeat apply conj; cbn; eauto; try easy.
-        * intros. destruct r; eauto; cbn; try constructor.
-          eapply Val.inject_ptr. unfold Mem.flat_inj. admit. admit. admit.
+        * intros.
+          assert (Val.inject (Mem.flat_inj (Mem.nextblock m)) (Vptr b Ptrofs.zero) (Vptr b Ptrofs.zero)).
+          { eapply Val.inject_ptr. unfold Mem.flat_inj.
+             destruct plt. reflexivity.
+             exfalso. apply n. erewrite init_mem_nextblock; eauto.
+             eapply Genv.genv_symb_range; eauto.
+             apply Genv.invert_find_symbol; eauto. reflexivity. }
+          destruct r; eauto; cbn; try constructor; eauto.
+          destruct i; eauto; cbn.
         * constructor; cbn.
           -- erewrite init_mem_nextblock; eauto. reflexivity.
-          -- intros x Hx.  admit.
-          -- constructor. unfold Mem.inject.
-             (* Search (Mem.inject _ ?m ?m). *)
-             (* Search Mem.inject_neutral. *)
-             admit.
+          -- intros x Hx. eapply init_mem_matches; eauto.
+          -- constructor. eapply initmem_inject; eauto.
       + cbn. repeat apply conj; eauto. constructor. eauto.
-        constructor; cbn.
-        (* Search (Genv.match_stbls _ ?se ?se). *)
-        admit. admit. admit.
+        constructor; cbn; erewrite init_mem_nextblock; eauto; try easy.
+        apply match_stbls_flat_inj.
       + intros. inv H2. exists (Some i). split; eauto.
         cbn in H0.
         destruct H0 as (r3 & Hr3 & HR). inv Hr3.
@@ -199,7 +377,8 @@ Section INIT_C_ASM.
         constructor. easy.
     - easy.
     - easy.
-  Admitted.
+    Unshelve. cbn. exact tt.
+  Qed.
 
 End INIT_C_ASM.
 
@@ -368,19 +547,248 @@ Section SYS_C_ASM.
 
   Local Transparent Archi.ptr64.
 
+  Require Import CallconvAlgebra CallConv CKLR.
+  Require Import Inject.
+  Require Import InjectFootprint.
+  Require Import Extends.
+  Require Import VAInject.
+  Require Import VAExtends.
+
+(* Definition cc_cklrs : callconv li_c li_c := *)
+(*   injp + inj + ext + vainj + vaext. *)
+
+  Inductive mm_cklr: ccworld cc_cklrs -> mem -> mem -> Prop :=
+  | mm_cklr_vaext w m m' (HM: match_mem vaext w m m'): mm_cklr (inr w) m m'
+  | mm_cklr_vainj w m m' (HM: match_mem vainj w m m'): mm_cklr (inl (inr w)) m m'
+  | mm_cklr_ext w m m' (HM: match_mem ext w m m'): mm_cklr (inl (inl (inr w))) m m'
+  | mm_cklr_inj w m m' (HM: match_mem inj w m m'): mm_cklr (inl (inl (inl (inr w)))) m m'
+  | mm_cklr_injp w m m' (HM: match_mem injp w m m'): mm_cklr (inl (inl (inl (inl w)))) m m'.
+
+  Inductive mp_cklr: ccworld cc_cklrs -> block -> ptrofs -> block -> ptrofs -> Prop :=
+  | mp_cklr_vaext w b ofs b' ofs'
+      (HP: ptr_inject (mi vaext w) (b, (Ptrofs.unsigned ofs)) (b', (Ptrofs.unsigned ofs'))):
+      mp_cklr (inr w) b ofs b' ofs'
+  | mp_cklr_vainj w b ofs b' ofs'
+      (HP: ptr_inject (mi vainj w) (b, (Ptrofs.unsigned ofs)) (b', (Ptrofs.unsigned ofs'))):
+      mp_cklr (inl (inr w)) b ofs b' ofs'
+  | mp_cklr_ext w b ofs b' ofs'
+      (HP: ptr_inject (mi ext w) (b, (Ptrofs.unsigned ofs)) (b', (Ptrofs.unsigned ofs'))):
+      mp_cklr (inl (inl (inr w))) b ofs b' ofs'
+  | mp_cklr_inj w b ofs b' ofs'
+      (HP: ptr_inject (mi inj w) (b, (Ptrofs.unsigned ofs)) (b', (Ptrofs.unsigned ofs'))):
+      mp_cklr (inl (inl (inl (inr w)))) b ofs b' ofs'
+  | mp_cklr_injp w b ofs b' ofs'
+      (HP: ptr_inject (mi injp w) (b, (Ptrofs.unsigned ofs)) (b', (Ptrofs.unsigned ofs'))):
+      mp_cklr (inl (inl (inl (inl w)))) b ofs b' ofs'.
+
+  Lemma inject_bytes j bytes y:
+    list_rel (memval_inject j) (map Byte bytes) y ->
+    y = map Byte bytes.
+  Proof.
+    revert y. induction bytes; intros; inv H; eauto.
+    cbn. f_equal.
+    - inv H2. reflexivity.
+    - eapply IHbytes. eauto.
+  Qed.
+
+  Lemma match_cklr_loadbytes w m b ofs m' b' ofs' len bytes:
+    mm_cklr w m m' ->
+    mp_cklr w b ofs b' ofs' ->
+    Mem.loadbytes m b (Ptrofs.unsigned ofs) len = Some (map Byte bytes) ->
+    Mem.loadbytes m' b' (Ptrofs.unsigned ofs') len = Some (map Byte bytes).
+  Proof.
+    intros Hm Hp Hl. inv Hm; inv Hp.
+    - exploit cklr_loadbytes; eauto. unfold k1, uncurry. rewrite Hl.
+      intros Ho. inv Ho. apply inject_bytes in H1. congruence.
+    - exploit cklr_loadbytes; eauto. unfold k1, uncurry. rewrite Hl.
+      intros Ho. inv Ho. apply inject_bytes in H1. congruence.
+    - exploit cklr_loadbytes; eauto. unfold k1, uncurry. rewrite Hl.
+      intros Ho. inv Ho. apply inject_bytes in H1. congruence.
+    - exploit cklr_loadbytes; eauto. unfold k1, uncurry. rewrite Hl.
+      intros Ho. inv Ho. apply inject_bytes in H1. congruence.
+    - exploit cklr_loadbytes; eauto. unfold k1, uncurry. rewrite Hl.
+      intros Ho. inv Ho. apply inject_bytes in H1. congruence.
+  Qed.
+
+  Hint Resolve ptr_ptrbits_inject_unsigned.
+
+  Lemma bytes_inject j bytes:
+    list_rel j (map Byte bytes) (map Byte bytes).
+  Proof.
+  Admitted.
+
+  Lemma match_cklr_storebytes w m1 m2 m3 b1 ofs1 b2 ofs2 bytes:
+    mm_cklr w m1 m2 ->
+    mp_cklr w b1 ofs1 b2 ofs2 ->
+    Mem.storebytes m1 b1 (Ptrofs.unsigned ofs1) (map Byte bytes) = Some m3 ->
+    exists wx m4, Mem.storebytes m2 b2 (Ptrofs.unsigned ofs2) (map Byte bytes) = Some m4
+             /\ mm_cklr wx m3 m4.
+  Proof.
+    intros Hm Hp Hs. inv Hm; inv Hp.
+    - exploit @cklr_storebytes; eauto.
+      apply ptrbits_rptr_inject_unsigned; eauto.
+      apply bytes_inject.
+      unfold k1, uncurry. rewrite Hs. intros. inv H.
+      destruct H2 as (wx & Hw & Hm).
+      eexists (inr wx), y. split; eauto. constructor. eauto.
+    - admit.
+    - admit.
+    - admit.
+    - admit.
+  Admitted.
+
+  Inductive mm_cklrs: ccworld (cc_cklrs^{*}) -> mem -> mem -> Prop :=
+  | mm_cklrs_zero m: mm_cklrs (existT _ 0%nat tt) m m
+  | mm_cklrs_succ n se w wn m1 m2 m3:
+        mm_cklr w m1 m2 -> mm_cklrs (existT _ n wn) m2 m3 ->
+        mm_cklrs (existT _ (S n) (se, w, wn)) m1 m3.
+
+  Inductive mp_cklrs: ccworld (cc_cklrs^{*}) -> block -> ptrofs -> block -> ptrofs -> Prop :=
+  | mp_cklrs_zero b ofs: mp_cklrs (existT _ 0%nat tt) b ofs b ofs
+  | mp_cklrs_succ n se w wn b1 ofs1 b2 ofs2 b3 ofs3:
+        mp_cklr w b1 ofs1 b2 ofs2 -> mp_cklrs (existT _ n wn) b2 ofs2 b3 ofs3 ->
+        mp_cklrs (existT _ (S n) (se, w, wn)) b1 ofs1 b3 ofs3.
+
+  Require Import Classical.
+
+  Ltac subst_dep :=
+    subst;
+    lazymatch goal with
+    | H: existT ?P ?x _ = existT ?P ?x _ |- _ =>
+        apply inj_pair2 in H; subst_dep
+    | _ => idtac
+    end.
+
+  (* Lemma match_cklrs_loadbytes n w m1 b1 ofs1 m2 b2 ofs2 len bytes: *)
+  (*   match_cklrs n w m1 b1 ofs1 m2 b2 ofs2 -> *)
+  (*   Mem.loadbytes m1 b1 ofs1 len = Some (map Byte bytes) -> *)
+  (*   Mem.loadbytes m2 b2 ofs2 len = Some (map Byte bytes). *)
+  (* Proof. *)
+  (*   revert w m1 b1 ofs1 m2 b2 ofs2 bytes. *)
+  (*   induction n; intros; inv H; eauto. *)
+  (*   subst_dep. eauto using match_cklr_loadbytes. *)
+  (* Qed. *)
+
+  Inductive mm_ca: ccworld (cc_cklrs^{*}) -> world inj -> mem -> mem -> Prop :=
+  | mm_ca_intro wn wi m1 m2 m3:
+    mm_cklrs wn m1 m2 -> match_mem inj wi m2 m3 -> mm_ca wn wi m1 m3.
+
+  Inductive mp_ca: ccworld (cc_cklrs^{*}) -> world inj -> block -> ptrofs -> block -> ptrofs -> Prop :=
+  | mp_ca_intro wn wi b1 ofs1 b2 ofs2 b3 ofs3:
+    mp_cklrs wn b1 ofs1 b2 ofs2 ->
+    ptr_inject (mi inj wi) (b2, (Ptrofs.unsigned ofs2)) (b3, (Ptrofs.unsigned ofs3)) ->
+    mp_ca wn wi b1 ofs1 b3 ofs3.
+
+  Lemma ca_storebytes n w m1 b1 ofs1 m2 b2 ofs2 bytes m3:
+    mm_ca n w m1 m2 ->
+    Mem.storebytes m2 b2 (Ptrofs.unsigned ofs2) (map Byte bytes) = Some m3 ->
+    exists m4, Mem.storebytes m1 b1 (Ptrofs.unsigned ofs1) (map Byte bytes) = Some m4
+          /\ mm_ca n w m4 m3.
+  Admitted.
+
+  Inductive match_sys_state:
+    ccworld (cc_cklrs^{*}) -> world inj -> sys_state -> sys_state -> Prop :=
+  | match_sys_state_read_query wn wi len b1 ofs1 m1 b2 ofs2 m2:
+      mm_ca wn wi m1 m2 ->
+      mp_ca wn wi b1 ofs1 b2 ofs2 ->
+      match_sys_state wn wi (sys_read_query len b1 ofs1 m1) (sys_read_query len b2 ofs2 m2)
+  | match_sys_state_read_reply wn wi bytes b1 ofs1 m1 b2 ofs2 m2:
+      mm_ca wn wi m1 m2 ->
+      mp_ca wn wi b1 ofs1 b2 ofs2 ->
+      match_sys_state wn wi (sys_read_reply bytes b1 ofs1 m1) (sys_read_reply bytes b2 ofs2 m2).
+
+  (*   Variant sys_state := *)
+  (*     | sys_read_query (n: int64) (b: block) (ofs: ptrofs) (m: mem) *)
+  (*     | sys_read_reply (bytes: list byte) (b: block) (ofs: ptrofs) (m: mem) *)
+  (*     | sys_write_query (bytes: list byte) (m: mem) *)
+  (*     | sys_write_reply (n: int) (m: mem). *)
+
+  Definition nw_of_world (w: ccworld cc_compcert): sigT (fun n => ccworld (cc_cklrs ^ n)).
+  Proof. cbn in w. destruct w. destruct p. exact s0. Defined.
+
+  Definition injw_of_world (w: ccworld cc_compcert): world inj.
+  Proof. cbn in w. eprod_crush. exact i. Defined.
+
+  Import ListNotations.
+
+  Lemma cklrs_match_query_inv (nw: ccworld (cc_cklrs ^ {*})) b ofs len m q vf:
+    match_query (cc_cklrs ^ {*}) nw
+                (cq vf rw_sig [Vint (Int.repr 0); Vptr b ofs; Vlong len] m)
+                q ->
+    exists m' b' ofs' vf',
+      q = (cq vf' rw_sig [Vint (Int.repr 0); Vptr b' ofs'; Vlong len] m')
+      /\ mm_cklrs nw m m' /\ mp_cklrs nw b ofs b' ofs'.
+  Proof.
+  Admitted.
+
+  Hypothesis (Hwin64: Archi.win64 = false).
+
+  Lemma free_empty: forall m b x m',
+      Mem.free m b x x = Some m' -> m = m'.
+  Proof.
+    intros. apply Mem.free_result in H. subst.
+    unfold Mem.unchecked_free. destruct m. cbn.
+    eapply Mem.mkmem_ext; eauto.
+    destruct mem_access. unfold PMap.set. cbn. f_equal.
+    induction t.
+    (* PTree.extensionality_empty *)
+  Admitted.
+
   Lemma sys_c_asm p tp:
     match_prog p tp -> forward_simulation 1 cc_compcert (sys_c p) (sys_asm tp).
   Proof.
     intros H. assert (Hsk: erase_program p = erase_program tp).
-    { apply clight_semantic_preservation in H as [H1 ?].
-      apply H1. }
+    eapply match_prog_skel; eauto.
     constructor. econstructor. apply Hsk.
     intros. reflexivity.
     intros. instantiate (1 := fun _ _ _ => _). cbn beta.
-    eapply forward_simulation_step with (match_states := eq).
+    set (ms := match_sys_state (nw_of_world wB) (injw_of_world wB)).
+    eapply forward_simulation_step with (match_states := fun s1 s2 => ms s1 s2).
     - intros. inv H3.
       + unfold cc_compcert in *. cbn in wB, H2 |- *.
-        eprod_crush. destruct s9. inv H3.
+        eprod_crush. destruct s9. inv H3. destruct H10; subst. cbn in *.
+        (* cklrs *)
+        eapply (cklrs_match_query_inv (existT _ x4 c0)) in H2 as
+            (mx & bx & ofsx & vfx & Hqx & Hmx & Hpx). subst x0.
+        (* lessdef *)
+        inv H5.
+        repeat match goal with
+        | [ H: Val.lessdef_list _ _ |- _ ] => inv H
+        | [ H: Val.lessdef _ _ |- _ ] => inv H
+        end.
+        (* cc_c_locset *)
+        inv H6.
+        (* cc_locset_mach: need to show args_removed changes nothing *)
+        inv H7.
+        inv H14. inv H2.
+        { admit. }
+        cbn in H2. rewrite Hwin64 in H2. cbn in H2. apply free_empty in H2. subst m1.
+        (* cc_mach_asm *)
+        inv H8.
+        (* cc_asm vainj *)
+        destruct q2. destruct H9. destruct H8.
+        (* arguments *)
+        cbn in H13. rewrite Hwin64 in H13. cbn in H13. inv H13.
+        assert (exists b' ofs', r0#RSI = Vptr b' ofs' /\ Val.inject i (Vptr bx ofsx) (Vptr b' ofs')) as (b' & ofs' & Hofs & Hb').
+        { admit. }
+        eexists (sys_read_query n b' ofs' m1). split.
+        * econstructor; eauto.
+          -- admit.
+          -- admit.
+          -- admit.
+          -- admit.
+        * constructor.
+          (* mem *)
+          -- econstructor; eauto. inv H9; auto.
+          (* ptr *)
+          -- econstructor; eauto. admit.
+             (* ptr_ptrbits_inject_unsigned *)
+      + admit.
+    - intros. inv H3.
+      + admit.
+
+
+
   Admitted.
 
 End SYS_C_ASM.
